geb-lean/GebLeanTests/Utilities/KArith.lean
@@ -10,3 +10,7 @@ open GebLean
 #guard KMor1.pred.interp ![0] == 0
 #guard KMor1.pred.interp ![1] == 0
 #guard KMor1.pred.interp ![5] == 4
+
+#guard KMor1.isZero.interp ![0] == 1
+#guard KMor1.isZero.interp ![1] == 0
+#guard KMor1.isZero.interp ![10] == 0
